\documentclass[11pt]{article}
%\usepackage{fullpage}
\usepackage{amsmath}
\usepackage{amsfonts}
\usepackage{graphicx}
\usepackage{caption}
\textheight=8.5in
\topmargin=0in
\headheight=0in
\headsep=0in
\oddsidemargin=0in
\evensidemargin=0in
\textwidth=6in
\linespread{1.2}
\title {\vspace*{-2em}Final Exam}
\author{Dingkang Wang}
\date {\today}

\begin{document}

\maketitle

\begin{equation}
    P(\mathbf{s}|\mathbf{o}) = \frac{1}{Z_{\mathbf{s}}} \exp \left( \sum_{t=1}^{T} \sum_{k} \lambda_k f_k(s_{t-1}, s_t, o_t) \right)
\end{equation}
\\

\begin{equation}
    Z_{\mathbf{s}} = \sum_{\mathbf{s}} \exp \left( \sum_{t=1}^{T} \sum_{k} \lambda_k f_k(s_{t-1}, s_t, o_t) \right)
\end{equation}
\\

\begin{equation}
    L = \sum_{n=1}^{N} \log P( \mathbf{s}^{(n)} | \mathbf{o}^{(n)}) - \sum_{k} \frac{\lambda_k^2}{2\sigma}
\end{equation}
\\

\begin{equation}
    \frac{\partial L}{\partial \lambda_k} = \sum_{n=1}^{N} \left( F_k ( \mathbf{s}^{(n)}, \mathbf{o}^{(n)} ) - \sum_{\mathbf{s}} P( \mathbf{s} | \mathbf{o}^{(n)}) F_k ( \mathbf{s}, \mathbf{o}^{(n)} ) \right)
\end{equation}
\\

\begin{equation}
    \sum_{\mathbf{s}} P( \mathbf{s} | \mathbf{o}^{(n)}) F_k ( \mathbf{s}, \mathbf{o}^{(n)} ) = E_{p(\mathbf{s}|\mathbf{o}^{(n)})} [ F_k(\mathbf{s}, \mathbf{o}^{(n)}) ]
\end{equation}
\\

\begin{equation}
     E_{p(\mathbf{s}|\mathbf{o}^{(n)})} [ F_k(\mathbf{s}, \mathbf{o}^{(n)}) ] = \frac{\sum_{t=1}^{T} \sum_{s_{t-1}, s_t} \alpha(t-1, s_{t-1}) f_k(s_{t-1}, s_{t}, o^{(n)}_t) \exp^{\lambda_k f_k(s_{t-1}, s_{t}, o^{(n)}_t)} \beta(t, s_t)}{Z_{\mathbf{s}}}
\end{equation}
\\

\begin{equation}
     Z_{\mathbf{s}} = \beta(1, 0) + \beta(1, 1) = \alpha(N, 0) + \alpha(N, 1)
\end{equation}
\\

\begin{equation}
V(t, s) = \left\{ \begin{array}{lc}
\max_{s'}( V(t-1, s') \exp \left( \sum_k \lambda_k f_k(s', s, \mathbf{o}_t) \right) ) & t>1 \\
s==1 & t=1
\end{array} \right.
\end{equation}
\\

\begin{equation}
V(t, s) = \left\{ \begin{array}{lc}
\max_{s'}( V(t-1, s') + \sum_k \lambda_k f_k(s', s, \mathbf{o}_t) ) & t>1 \\
V(1,0) = -\infty,\ V(1, 1) = 0 & t=1
\end{array} \right.
\end{equation}
\\

\begin{equation}
    \alpha(t, s) = \sum_{s'} \alpha(t-1, s') \exp \left( \sum_k \lambda_k f_k(s', s, \mathbf{o}_t) \right)
\end{equation}
\\

\begin{equation}
    \beta(t, s) = \sum_{s'} \beta(t+1, s') \exp \left( \sum_k \lambda_k f_k(s, s', \mathbf{o}_{t+1}) \right)
\end{equation}
\\

\end{document} 